pt_inv pas_refined
Signed-off-by: Ryan Barry <ryan.barry@unsw.edu.au>

proof/access-control/RISCV64/ArchCNode_AC.thy
@@ -351,6 +351,7 @@ lemma pas_refined_arch_state_update_not_asids[simp]:
  "riscv_asid_table (f (arch_state s)) = riscv_asid_table (arch_state s)
   \<Longrightarrow> pas_refined aag (arch_state_update f s) = pas_refined aag s"
   apply (auto simp add: pas_refined_def state_objs_to_policy_def)
+apply (erule subsetD)
   sorry
 
 crunch cdt[wp]: store_pte "\<lambda>s. P (cdt s)"
@@ -363,49 +364,1850 @@ lemma store_pte_state_refs[wp]:
                  elim!: rsubst[where P=P, OF _ ext])
   done
 
+(* FIXME ryanb - remove? *)
 lemma all_rsubst:
   "\<lbrakk> \<forall>v. P (f v); \<exists>v. f v = r \<rbrakk> \<Longrightarrow> P r"
   by clarsimp
 
-lemma store_pte_st_vrefs[wp]:
-  "\<lbrace>\<lambda>s. \<forall>S. P ((state_vrefs s) (p && ~~ mask pt_bits :=
-                                  (state_vrefs s (p && ~~ mask pt_bits) - S) \<union>
-                                  (\<Union>(p', sz, auth)\<in>set_option (pte_ref2 level pte).
-                                     (\<lambda>(p'', a). (p'', (p && mask pt_bits) >> 2, APageTable, a)) `
-                                                                       (ptr_range p' sz \<times> auth))))\<rbrace>
-   store_pte p pte
-   \<lbrace>\<lambda>rv s. P (state_vrefs s)\<rbrace>"
-  sorry
-(* FIXME ryanb
-  apply (simp add: store_pte_def set_pt_def set_object_def)
-  apply (wp get_object_wp)
-  apply (clarsimp simp: state_vrefs_def vs_refs_aux_def obj_at_def)
-  apply (simp add: fun_upd_def[symmetric] fun_upd_comp)
-  apply (erule all_rsubst[where P=P])
-  apply (subst fun_eq_iff, clarsimp simp: split_def)
-  apply (cases "pte_ref2 level pte")
-   apply (auto simp: ucast_ucast_mask shiftr_over_and_dist
-                     word_bw_assocs mask_def pt_bits_def pageBits_def)
+
+
+lemma "\<lbrace>valid_pti pti\<rbrace> perform_page_table_invocation pti \<lbrace>Q\<rbrace>"
+apply (unfold perform_page_table_invocation_def perform_pt_inv_map_def perform_pt_inv_unmap_def)
+apply (case_tac pti; clarsimp simp: valid_pti_def)
+apply (rename_tac acap cslot_a cslot_b pte pt_slot)
+thm valid_vspace_objs_def
+term wellformed_pte
+term perform_page_table_invocation
+term perform_pt_inv_map
+term valid_pti
+term invalid_pte_at
+oops
+
+lemma "\<lbrace>valid_pti pti\<rbrace> perform_page_table_invocation pti \<lbrace>Q\<rbrace>"
+apply (unfold perform_page_table_invocation_def perform_pt_inv_map_def perform_pt_inv_unmap_def)
+apply (case_tac pti; clarsimp simp: valid_pti_def)
+subgoal sorry
+apply (rename_tac acap cslot_a cslot_b)
+thm valid_vspace_objs_def
+term wellformed_pte
+term perform_page_table_invocation
+term perform_pt_inv_map
+term valid_pti
+term invalid_pte_at
+oops
+
+
+
+lemma vs_lookup_PageTablePTE:
+  "\<lbrakk> pspace_aligned s; valid_vspace_objs s; valid_asid_table s;
+     invalid_pte_at p s; ptes_of s' = ptes_of s (p \<mapsto> pte); is_PageTablePTE pte;
+     asid_pools_of s' = asid_pools_of s; asid_table s' = asid_table s;
+     vref \<in> user_region; vs_lookup_table level asid vref s' = Some (lvl', pt);
+     pts_of s (the (pte_ref pte)) = Some empty_pt; pt \<noteq> pptr_from_pte pte \<rbrakk>
+     \<Longrightarrow> \<exists>level' \<ge> level. vs_lookup_table level' asid vref s = Some (lvl', pt)"
+  apply (induct level arbitrary: lvl' pt rule: bit0.from_top_full_induct[where y=max_pt_level])
+   apply (fastforce simp: geq_max_pt_level vs_lookup_table_def pool_for_asid_def obind_def)
+  apply (rule_tac x=lvl' in exI)
+  apply (rule context_conjI)
+   apply (fastforce dest: vs_lookup_min_level)
+  apply (drule vs_lookup_level)
+  apply (case_tac "lvl' < max_pt_level")
+   apply (frule vs_lookup_table_split_last_Some; clarsimp)
+   apply (erule_tac x="lvl'+1" in allE)
+   apply (drule mp)
+    apply (fastforce elim: le_less_trans dest: vm_level_less_plus_1_mono)
+   apply (erule_tac x="lvl'+1" in allE)
+   apply clarsimp
+   apply (frule subst[where s="ptes_of s'" and P="\<lambda>ptes. ptes _ = _"])
+    apply assumption
+   apply (drule mp, fastforce simp: pte_ref_def2 ptes_of_Some split: if_splits)
+   apply (cases pte; clarsimp)
+   apply (drule_tac bot_level=level' in vs_lookup_level)
+   apply (subst vs_lookup_split_Some)
+     prefer 3
+     apply (rule exI, rule conjI, assumption)
+     apply (frule_tac P="\<lambda>x. x" and level1=lvl' and level'1="lvl'+1"
+                   in subst[OF vs_lookup_split_Some, rotated 2])
+       apply (fastforce dest: vm_level_less_le_1)
+      apply (fastforce dest: vm_level_less_max_pt_level vm_level_less_plus_1_mono)
+     apply clarsimp
+     apply (subst (asm) pt_walk.simps)
+     apply (clarsimp simp: obind_def)
+     apply (subst pt_walk.simps)
+     apply (clarsimp split: if_splits simp: obind_def)
+    apply (fastforce dest: vm_level_less_le_1)
+   apply (fastforce dest: vm_level_less_max_pt_level vm_level_less_plus_1_mono)
+  apply (case_tac "lvl' = asid_pool_level")
+   apply (auto simp: geq_max_pt_level vs_lookup_table_def pool_for_asid_def obind_def)
   done
-*)
+
+lemma vs_lookup_PageTablePTE':
+  "\<lbrakk> pspace_aligned s; valid_vspace_objs s; valid_asid_table s;
+     invalid_pte_at p s; ptes_of s' = ptes_of s (p \<mapsto> pte); is_PageTablePTE pte;
+     asid_pools_of s' = asid_pools_of s; asid_table s' = asid_table s;
+     vref \<in> user_region; vs_lookup_table level asid vref s = Some (lvl', pt) \<rbrakk>
+     \<Longrightarrow> \<exists>level' \<ge> level. vs_lookup_table level' asid vref s' = Some (lvl', pt)"
+  apply (induct level arbitrary: lvl' pt rule: bit0.from_top_full_induct[where y=max_pt_level])
+   apply (fastforce simp: geq_max_pt_level vs_lookup_table_def pool_for_asid_def obind_def)
+  apply (rule_tac x=lvl' in exI)
+  apply (rule context_conjI)
+   apply (fastforce dest: vs_lookup_min_level)
+  apply (drule vs_lookup_level)
+  apply (case_tac "lvl' < max_pt_level")
+   apply (frule vs_lookup_table_split_last_Some; clarsimp)
+   apply (erule_tac x="lvl'+1" in allE)
+   apply (drule mp)
+    apply (fastforce elim: le_less_trans dest: vm_level_less_plus_1_mono)
+   apply (erule_tac x="lvl'+1" in allE)
+   apply clarsimp
+   apply (drule_tac bot_level=level' in vs_lookup_level)
+   apply (subst vs_lookup_split_Some)
+     prefer 3
+     apply (rule exI, rule conjI, assumption)
+     apply (frule_tac P="\<lambda>x. x" and level1=lvl' and level'1="lvl'+1"
+                   in subst[OF vs_lookup_split_Some, rotated 2])
+       apply (fastforce dest: vm_level_less_le_1)
+      apply (fastforce dest: vm_level_less_max_pt_level vm_level_less_plus_1_mono)
+     apply clarsimp
+     apply (subst (asm) pt_walk.simps)
+     apply (clarsimp simp: obind_def split: if_splits)
+     apply (subst pt_walk.simps)
+     apply (clarsimp simp: obind_def split: if_splits)
+     apply (cases pte; clarsimp)
+     apply (frule is_aligned_pt[rotated])
+      apply (erule vs_lookup_table_pt_at; fastforce)
+     apply (clarsimp simp: invalid_pte_at_def ptes_of_Some pts_of_Some aobjs_of_Some)
+    apply (fastforce dest: vm_level_less_le_1)
+   apply (fastforce dest: vm_level_less_max_pt_level vm_level_less_plus_1_mono)
+  apply (case_tac "lvl' = asid_pool_level")
+   apply (auto simp: geq_max_pt_level vs_lookup_table_def pool_for_asid_def obind_def)
+  done
+
+
+lemma vs_lookup_slot_table_base':
+  "\<lbrakk> vs_lookup_slot level asid vref s = Some (level, slot); vref \<in> user_region;
+     level \<le> max_pt_level; invs s \<rbrakk> \<Longrightarrow>
+   slot = pt_slot_offset level (table_base slot) vref"
+  apply (clarsimp simp: vs_lookup_slot_def split: if_split_asm)
+  apply (drule vs_lookup_table_is_aligned; clarsimp)
+  done
+
+
+lemma level_of_slot_vs_lookup_slot:
+  "\<lbrakk> vs_lookup_slot level asid vref s = Some (level, p);
+     ptes_of s p = Some pte; level \<le> max_pt_level; vref \<in> user_region; invs s \<rbrakk>
+     \<Longrightarrow> level_of_slot asid vref p s = level"
+apply (subst level_of_slot_def)
+apply (rule Greatest_equality)
+apply clarsimp
+thm vs_lookup_slot_no_asid vs_lookup_slot_unique_level
+    apply (case_tac "y = asid_pool_level")
+apply clarsimp
+apply (drule vs_lookup_slot_no_asid)
+apply simp
+apply clarsimp+
+
+apply (drule (1) vs_lookup_slot_unique_level)
+apply fastforce+
+done
+
+
+lemma state_vrefs_store_NonPageTablePTE:
+  "\<lbrakk> invs s; is_aligned p pte_bits; vs_lookup_slot level asid vref s = Some (level, p);
+     vref \<in> user_region; pte = InvalidPTE;
+     kheap s (table_base p) = Some (ArchObj (PageTable pt)) \<rbrakk>
+     \<Longrightarrow> state_vrefs (s\<lparr>kheap := \<lambda>a. if a = table_base p
+                                     then Some (ArchObj (PageTable (\<lambda>a. if a = table_index p then pte else pt a)))
+                                     else kheap s a\<rparr>) =
+         (\<lambda>x. if \<exists>level' vref'. vref' \<in> user_region \<and> vref_for_level vref' (level + 1) = vref_for_level vref (level + 1) \<and>
+                                p = pt_slot_offset level (table_base p) vref' \<and>
+                                pt_walk level level' (table_base p) vref' (ptes_of s) = Some (level',x)
+              then (if x = table_base p
+                    then vs_refs_aux level (PageTable (\<lambda>a. if a = table_index p then pte else pt a))
+                    else {})
+              else state_vrefs s x)"
+  apply (rule all_ext)
+
+  apply (case_tac "level = asid_pool_level")
+   apply (clarsimp simp: vs_lookup_slot_def split: if_splits)
+   apply (clarsimp simp: vs_lookup_table_def split: if_splits)
+   apply (drule pool_for_asid_no_pte)
+      apply (simp add: ptes_of_Some pts_of_Some aobjs_of_Some)
+     apply fastforce
+    apply fastforce
+   apply fastforce
+
+apply (prop_tac "ptes_of s p \<noteq> None")
+apply (drule valid_vspace_objs_strong_slotD)
+apply fastforce+
+
+  apply (frule vs_lookup_slot_table_base')
+     apply fastforce+
+  apply (drule vs_lookup_slot_table_base)
+     apply fastforce+
+
+  apply safe
+
+
+(* first thing *)
+   apply (subst (asm) state_vrefs_def opt_map_def)+
+   apply (clarsimp split: option.splits split del: if_split)
+   apply (clarsimp split: if_split_asm option.splits split del: if_split)
+(* x = table_base p *)
+    apply (subst (asm) vs_lookup_non_PageTablePTE[where s=s and p=p and pte=pte])
+           apply (clarsimp simp: ptes_of_Some pts_of_Some aobjs_of_Some)
+          apply (rule all_ext)
+          apply (clarsimp simp: opt_map_def pte_of_def obind_def)
+          apply (fastforce dest: pte_ptr_eq)
+         apply simp
+        apply (fastforce simp: opt_map_def)
+       apply (fastforce simp: opt_map_def)
+      apply fastforce+
+    (* done *)
+
+    apply (clarsimp split: if_splits)
+
+
+     apply (rule conjI)
+      prefer 2
+      apply clarsimp
+      apply (erule_tac x=level in allE)
+      apply (erule_tac x=vref in allE)
+      apply clarsimp
+
+     apply (drule vs_lookup_level) back
+
+     apply (case_tac "lvl = asid_pool_level")
+      apply clarsimp
+      apply (frule vs_lookup_table_no_asid)
+         apply (fastforce simp: ptes_of_Some pts_of_Some aobjs_of_Some)
+        apply fastforce
+       apply fastforce
+      apply fastforce
+
+     apply clarsimp
+     apply (drule (1) vs_lookup_table_unique_level)
+           apply fastforce+
+
+    apply (rule conjI)
+     prefer 2
+     apply clarsimp
+     apply (erule_tac x=level in allE) back
+     apply clarsimp
+
+     apply (drule vs_lookup_level) back
+
+     apply (case_tac "lvl = asid_pool_level")
+      apply clarsimp
+      apply (frule vs_lookup_table_no_asid)
+         apply (fastforce simp: ptes_of_Some pts_of_Some aobjs_of_Some)
+        apply fastforce
+       apply fastforce
+      apply fastforce
+
+     apply clarsimp
+     apply (drule (1) vs_lookup_table_unique_level)
+           apply fastforce+
+(* x \<noteq> table_base p *)
+
+
+   apply (subst (asm) vs_lookup_non_PageTablePTE[where s=s and p=p and pte=pte])
+          apply (clarsimp simp: ptes_of_Some pts_of_Some aobjs_of_Some)
+         apply (rule all_ext)
+         apply (clarsimp simp: opt_map_def pte_of_def obind_def)
+         apply (fastforce dest: pte_ptr_eq)
+        apply simp
+       apply (fastforce simp: opt_map_def)
+      apply (fastforce simp: opt_map_def)
+     apply fastforce+
+    (* done *)
+
+   apply (subst state_vrefs_def)
+   apply (clarsimp split: if_splits)
+
+  apply (case_tac "level' = asid_pool_level")
+      apply clarsimp
+      apply (frule vs_lookup_slot_no_asid)
+         apply (fastforce simp: ptes_of_Some pts_of_Some aobjs_of_Some)
+        apply fastforce
+       apply fastforce
+      apply fastforce
+    apply clarsimp
+
+    apply (prop_tac "level_of_slot asida vrefa p s = level'")
+apply (erule level_of_slot_vs_lookup_slot)
+apply (fastforce simp: ptes_of_Some pte_of_def obind_def pts_of_Some aobjs_of_Some split: option.splits)
+apply fastforce+
+
+    apply (subst (asm) vs_lookup_slot_table_unfold; fastforce)
+
+   apply (rule conjI)
+    prefer 2
+    apply (fastforce simp: opt_map_def)
+   apply clarsimp
+
+
+   apply (case_tac "level' < level")
+    prefer 2
+    apply (subst (asm) pt_walk.simps)
+    apply clarsimp
+
+
+apply (prop_tac "vs_lookup_slot level asid vref s = Some (level, p)")
+apply (fastforce simp: vs_lookup_slot_table_unfold)
+
+
+   apply (subst (asm) vs_lookup_vref_for_level_eq1)
+    apply (rule sym)
+    apply assumption
+
+
+   apply (frule (2) vs_lookup_table_extend)
+
+   apply (frule vs_lookup_min_level) back
+   apply (drule vs_lookup_level) back
+
+
+    apply (case_tac "lvl = asid_pool_level")
+     apply (drule vs_lookup_table_pt_at) back
+          apply fastforce+
+         apply clarsimp
+         apply (frule vs_lookup_asid_pool)
+          apply fastforce
+         apply (clarsimp simp: asid_pools_of_ko_at obj_at_def)
+
+         apply (drule (1) vs_lookup_table_unique_level, rule refl)
+         apply fastforce+
+
+         apply clarsimp
+         apply (prop_tac "level' + 1 \<le> level")
+          apply (fastforce simp: bit0.plus_one_leq)
+
+
+         apply (erule_tac x=level in allE)
+         apply (drule mp)
+
+          apply (subst vs_lookup_slot_vref_for_level[symmetric])
+           apply assumption
+          apply (simp only:)
+          apply (subst vs_lookup_slot_vref_for_level)
+           apply assumption
+          apply (fastforce simp: vs_lookup_slot_table_unfold)
+          apply fastforce
+
+
+(* second bit *)
+
+apply (clarsimp simp: obind_def split: if_splits option.splits)
+
+(* second thing *)
+
+  apply (clarsimp simp: state_vrefs_def opt_map_def)
+
+apply (intro exI conjI)
+apply (rule refl)
+apply (subst vs_lookup_non_PageTablePTE[where s=s and p=p and pte=pte ])
+apply (clarsimp simp: ptes_of_Some pts_of_Some aobjs_of_Some)
+ apply (rule all_ext)
+        apply (clarsimp simp: opt_map_def pte_of_def obind_def)
+        apply (fastforce dest: pte_ptr_eq)
+       apply simp
+      apply (fastforce simp: opt_map_def)
+     apply (fastforce simp: opt_map_def)
+    apply fastforce
+    apply fastforce
+defer
+apply fastforce
+apply fastforce
+apply fastforce
+defer
+apply (clarsimp split: if_splits)
+apply auto[1]
+
+
+apply (prop_tac "level_of_slot asid vref p s = level")
+apply (subst level_of_slot_def)
+
+apply (rule Greatest_equality)
+apply (clarsimp simp: vs_lookup_slot_def obind_def)
+
+ apply (case_tac "ya = asid_pool_level")
+    (* lvla = asid_pool_level *)
+    apply clarsimp
+    apply (frule vs_lookup_slot_no_asid)
+         apply (clarsimp simp: ptes_of_Some pts_of_Some aobjs_of_Some pte_of_def obind_def split: option.splits)
+apply fastforce
+apply fastforce
+apply fastforce
+apply clarsimp
+apply clarsimp
+
+apply (subst (asm) vs_lookup_slot_table_unfold) back
+apply fastforce+
+
+apply clarsimp
+apply (drule (1) vs_lookup_table_unique_level)
+apply fastforce+
+
+apply (clarsimp simp: state_vrefs_def)
+apply (subst opt_map_def)
+apply (case_tac "x = table_base p"; clarsimp)
+
+apply (rule exI, rule conjI)
+prefer 2
+apply assumption
+apply (rule exI)+
+apply (rule conjI, rule refl)
+apply (clarsimp simp: aobjs_of_Some)
+apply (erule_tac x=level in allE)
+apply (erule_tac x=vref in allE)
+apply clarsimp
+
+apply (rule exI, rule conjI)
+prefer 2
+apply assumption
+apply (rule exI)+
+apply (rule conjI, rule refl)
+apply (clarsimp simp: aobjs_of_Some)
+
+apply (case_tac "lvl < level")
+
+apply (drule vs_lookup_level) back
+apply (subst (asm) vs_lookup_split_Some[where level'=level]) back
+apply fastforce
+apply fastforce
+apply clarsimp
+
+apply (rule_tac x=lvl in exI)
+apply (rule_tac x=asida in exI)
+apply (rule_tac x=vrefa in exI)
+
+
+apply (subst vs_lookup_non_PageTablePTE[where s=s and p=p and pte=pte ])
+apply (clarsimp simp: ptes_of_Some pts_of_Some aobjs_of_Some)
+ apply (rule all_ext)
+        apply (clarsimp simp: opt_map_def pte_of_def obind_def)
+        apply (fastforce dest: pte_ptr_eq)
+       apply simp
+      apply (fastforce simp: opt_map_def)
+     apply (fastforce simp: opt_map_def)
+    apply fastforce
+    apply fastforce
+  apply (clarsimp split: if_splits)
+  apply (intro conjI; clarsimp)
+prefer 2
+  using vs_lookup_table_extend apply blast
+
+    apply (case_tac "level' = asid_pool_level")
+     apply (fastforce dest: vs_lookup_slot_no_asid
+                       simp: ptes_of_Some pts_of_Some aobjs_of_Some pte_of_def obind_def split: option.splits)
+   apply clarsimp
+
+apply (prop_tac "level_of_slot asida vrefa p s = level'")
+
+apply (subst level_of_slot_def)
+apply (rule Greatest_equality)
+apply clarsimp
+
+    apply (case_tac "ya = asid_pool_level")
+     apply (fastforce dest: vs_lookup_slot_no_asid
+                       simp: ptes_of_Some pts_of_Some aobjs_of_Some pte_of_def obind_def split: option.splits)
+   apply clarsimp
+
+apply (drule (1) vs_lookup_slot_unique_level)
+apply fastforce+
+
+apply (simp only:)
+apply (thin_tac "level_of_slot _ _ _ _ = _")
+
+apply (subst (asm) vs_lookup_slot_table_unfold)
+apply fastforce+
+apply clarsimp
+apply (drule (1) vs_lookup_table_unique_level) back
+apply fastforce+
+
+
+apply (rule_tac x=lvl in exI)
+apply (rule_tac x=asida in exI)
+apply (rule_tac x=vrefa in exI)
+apply clarsimp
+
+
+apply (subst vs_lookup_non_PageTablePTE[where s=s and p=p and pte=pte ])
+apply (clarsimp simp: ptes_of_Some pts_of_Some aobjs_of_Some)
+ apply (rule all_ext)
+        apply (clarsimp simp: opt_map_def pte_of_def obind_def)
+        apply (fastforce dest: pte_ptr_eq)
+       apply simp
+      apply (fastforce simp: opt_map_def)
+     apply (fastforce simp: opt_map_def)
+    apply fastforce
+    apply fastforce
+apply (case_tac "\<exists>level'. vs_lookup_slot level' asida vrefa s = Some (level', p) \<and> lvl < level'"; clarsimp)
+
+prefer 2
+apply (fastforce dest: vs_lookup_level)
+apply (case_tac "level' = asid_pool_level")
+apply clarsimp
+apply (frule vs_lookup_slot_no_asid)
+         apply (clarsimp simp: ptes_of_Some pts_of_Some aobjs_of_Some pte_of_def obind_def split: option.splits)
+apply fastforce
+apply fastforce
+apply fastforce
+apply clarsimp
+apply clarsimp
+
+apply (prop_tac "level_of_slot asida vrefa p s = level'")
+apply (erule level_of_slot_vs_lookup_slot)
+apply fastforce+
+apply (simp only:)
+apply (thin_tac "level_of_slot _ _ _ _ = _")
+
+apply (clarsimp simp: vs_lookup_slot_def split: if_splits)
+  by (metis vs_lookup_slot_table vs_lookup_slot_unique_level)
+
+
+definition level_of_table :: "obj_ref \<Rightarrow> 'z::state_ext state \<Rightarrow> vm_level"
+  where
+  "level_of_table p s \<equiv>
+     GREATEST level. \<exists>asid vref. vref \<in> user_region \<and> vs_lookup_table level asid vref s = Some (level, p)"
+
+lemma level_of_table_vs_lookup_table:
+  "\<lbrakk> vs_lookup_table level asid vref s = Some (level, p);
+     ptes_of s p = Some pte; level \<le> max_pt_level; vref \<in> user_region; invs s \<rbrakk>
+     \<Longrightarrow> level_of_table p s = level"
+apply (subst level_of_table_def)
+apply (rule Greatest_equality)
+apply fastforce
+apply clarsimp
+thm vs_lookup_slot_no_asid vs_lookup_slot_unique_level
+    apply (case_tac "y = asid_pool_level")
+apply clarsimp
+apply (drule vs_lookup_table_no_asid)
+apply simp
+apply clarsimp+
+
+apply (drule (1) vs_lookup_table_unique_level)
+apply fastforce+
+done
+
+
+lemma state_vrefs_store_NonPageTablePTE':
+  "\<lbrakk> invs s; is_aligned p pte_bits; \<forall>level asid vref. vref \<in> user_region \<longrightarrow> vs_lookup_slot level asid vref s \<noteq> Some (level, p);
+      pte = InvalidPTE;
+     kheap s (table_base p) = Some (ArchObj (PageTable pt)) \<rbrakk>
+     \<Longrightarrow> state_vrefs (s\<lparr>kheap := \<lambda>a. if a = table_base p
+                                     then Some (ArchObj (PageTable (\<lambda>a. if a = table_index p then pte else pt a)))
+                                     else kheap s a\<rparr>) =
+         (\<lambda>x. if x = table_base p \<and> (\<exists>level. \<exists>\<rhd> (level, table_base p) s)
+                    then vs_refs_aux (level_of_table (table_base p) s) (PageTable (\<lambda>a. if a = table_index p then pte else pt a))
+              else state_vrefs s x)"
+  apply (rule all_ext)
+  apply safe
+
+
+(* first thing *)
+   apply (subst (asm) state_vrefs_def opt_map_def)+
+   apply (clarsimp split: option.splits split del: if_split)
+   apply (clarsimp split: if_split_asm option.splits split del: if_split)
+
+(* x = table_base p *)
+    apply (subst (asm) vs_lookup_non_PageTablePTE[where s=s and p=p and pte=pte])
+           apply (clarsimp simp: ptes_of_Some pts_of_Some aobjs_of_Some)
+          apply (rule all_ext)
+          apply (clarsimp simp: opt_map_def pte_of_def obind_def)
+          apply (fastforce dest: pte_ptr_eq)
+         apply simp
+        apply (fastforce simp: opt_map_def)
+       apply (fastforce simp: opt_map_def)
+      apply fastforce+
+    (* done *)
+
+    apply (clarsimp split: if_splits)
+apply safe
+
+    apply (case_tac "level = asid_pool_level")
+         apply (fastforce dest: vs_lookup_table_no_asid
+                          simp: ptes_of_Some pts_of_Some aobjs_of_Some pte_of_def obind_def
+                         split: option.splits)
+    apply (case_tac "lvl = asid_pool_level")
+      apply (drule vs_lookup_level)
+      apply (fastforce dest: vs_lookup_table_no_asid
+                       simp: ptes_of_Some pts_of_Some aobjs_of_Some pte_of_def obind_def
+                      split: option.splits)
+
+
+apply (prop_tac "level_of_table (table_base p) s = level")
+
+apply (erule level_of_table_vs_lookup_table)
+apply (fastforce simp: ptes_of_Some pte_of_def obind_def pts_of_Some aobjs_of_Some split: option.splits)
+apply fastforce+
+
+apply clarsimp
+apply (drule vs_lookup_level)
+apply (drule (1) vs_lookup_table_unique_level)
+apply fastforce
+apply fastforce
+apply fastforce
+apply fastforce
+apply fastforce
+apply fastforce
+apply fastforce
+apply (fastforce dest: vs_lookup_level)
+
+
+(* x = table_base p *)
+    apply (subst (asm) vs_lookup_non_PageTablePTE[where s=s and p=p and pte=pte])
+           apply (clarsimp simp: ptes_of_Some pts_of_Some aobjs_of_Some)
+          apply (rule all_ext)
+          apply (clarsimp simp: opt_map_def pte_of_def obind_def)
+          apply (fastforce dest: pte_ptr_eq)
+         apply simp
+        apply (fastforce simp: opt_map_def)
+       apply (fastforce simp: opt_map_def)
+      apply fastforce+
+    (* done *)
+    apply (clarsimp split: if_splits)
+apply (clarsimp simp: state_vrefs_def)
+apply (fastforce simp: aobjs_of_Some)
+
+
+
+apply (clarsimp split: if_splits)
+
+
+    apply (case_tac "level = asid_pool_level")
+         apply (fastforce dest: vs_lookup_table_no_asid
+                          simp: ptes_of_Some pts_of_Some aobjs_of_Some pte_of_def obind_def
+                         split: option.splits)
+
+apply (prop_tac "level_of_table (table_base p) s = level")
+apply (erule level_of_table_vs_lookup_table)
+apply (fastforce simp: ptes_of_Some pte_of_def obind_def pts_of_Some aobjs_of_Some split: option.splits)
+apply fastforce+
+
+apply (simp only:)
+apply (thin_tac "level_of_table _ _ = _")
+
+  apply (clarsimp simp: state_vrefs_def opt_map_def)
+
+apply (intro exI conjI)
+apply (rule refl)
+apply (subst vs_lookup_non_PageTablePTE[where s=s and p=p and pte=pte ])
+apply (clarsimp simp: ptes_of_Some pts_of_Some aobjs_of_Some)
+ apply (rule all_ext)
+        apply (clarsimp simp: opt_map_def pte_of_def obind_def)
+        apply (fastforce dest: pte_ptr_eq)
+       apply simp
+      apply (fastforce simp: opt_map_def)
+     apply (fastforce simp: opt_map_def)
+    apply fastforce
+    apply fastforce
+defer
+apply fastforce
+apply fastforce
+apply fastforce
+defer
+apply (clarsimp split: if_splits)
+apply auto[1]
+
+apply (case_tac "x = table_base p"; clarsimp)
+apply (clarsimp simp: state_vrefs_def)
+apply (fastforce dest: vs_lookup_level)
+
+  apply (clarsimp simp: state_vrefs_def opt_map_def)
+
+apply (intro exI conjI)
+apply (rule refl)
+apply (subst vs_lookup_non_PageTablePTE[where s=s and p=p and pte=pte ])
+apply (clarsimp simp: ptes_of_Some pts_of_Some aobjs_of_Some)
+ apply (rule all_ext)
+        apply (clarsimp simp: opt_map_def pte_of_def obind_def)
+        apply (fastforce dest: pte_ptr_eq)
+       apply simp
+      apply (fastforce simp: opt_map_def)
+     apply (fastforce simp: opt_map_def)
+    apply fastforce
+    apply fastforce
+defer
+apply fastforce
+apply fastforce
+apply fastforce
+defer
+apply (clarsimp split: if_splits)
+apply auto[1]
+done
+
+
+
+lemma state_vrefs_store_NonPageTablePTE_wp':
+"\<lbrace>\<lambda>s. invs s \<and> pte = InvalidPTE \<and>
+
+(\<forall>pt. ako_at (PageTable pt) (table_base p) s \<longrightarrow> is_aligned p pte_bits \<longrightarrow>
+ (if \<exists>level asid vref. vs_lookup_slot level asid vref s = Some (level, p) \<and> vref \<in> user_region
+  then (\<exists>level asid vref. vs_lookup_slot level asid vref s = Some (level, p) \<and> vref \<in> user_region \<and>
+                          P (\<lambda>x. (if \<exists>level' vref'. vref' \<in> user_region \<and> vref_for_level vref' (level + 1) = vref_for_level vref (level + 1) \<and>
+                                                    p = pt_slot_offset level (table_base p) vref' \<and>
+                                                    pt_walk level level' (table_base p) vref' (ptes_of s) = Some (level',x)
+                                  then (if x = table_base p
+                                        then vs_refs_aux level (PageTable (\<lambda>a. if a = table_index p then pte else pt a))
+                                        else {})
+                                  else state_vrefs s x)))
+else P (\<lambda>x. (if x = table_base p \<and> (\<exists>level. \<exists>\<rhd> (level, table_base p) s)
+                    then vs_refs_aux (level_of_table (table_base p) s) (PageTable (\<lambda>a. if a = table_index p then pte else pt a))
+              else state_vrefs s x))))
+\<rbrace> store_pte p pte \<lbrace>\<lambda>_ s. P (state_vrefs s)\<rbrace>"
+unfolding store_pte_def set_pt_def
+apply (wpsimp wp: set_object_wp)
+apply (case_tac "\<exists>level asid vref.
+                           vs_lookup_slot level asid vref s = Some (level, p) \<and> vref \<in> user_region")
+apply (erule_tac x=pt in allE)
+apply clarsimp
+apply (clarsimp simp: fun_upd_def)
+apply (subst state_vrefs_store_NonPageTablePTE)
+apply fastforce+
+apply (clarsimp simp: obj_at_def)
+apply (case_tac "level = asid_pool_level")
+     apply (fastforce dest: vs_lookup_slot_no_asid
+                      simp: ptes_of_Some pts_of_Some aobjs_of_Some pte_of_def obind_def obj_at_def
+                      split: option.splits)
+
+apply (case_tac "levela = asid_pool_level")
+     apply (fastforce dest: vs_lookup_slot_no_asid
+                      simp: ptes_of_Some pts_of_Some aobjs_of_Some pte_of_def obind_def obj_at_def
+                      split: option.splits)
+apply (drule (1) vs_lookup_slot_unique_level)
+apply fastforce+
+apply clarsimp
+apply (prop_tac "vref_for_level vrefa (level+1) = vref_for_level vref (level+1)")
+  apply (metis (mono_tags, hide_lams) vs_lookup_slot_table_base vs_lookup_slot_vref_for_level_eq vs_lookup_table_unique_level)
+apply clarsimp
+
+apply clarsimp
+apply (erule_tac x=pt in allE)
+apply (clarsimp simp: fun_upd_def)
+apply (subst state_vrefs_store_NonPageTablePTE')
+apply fastforce+
+apply (clarsimp simp: obj_at_def)
+apply clarsimp
+done
+
+
+
+lemma state_vrefs_store_NonPageTablePTE_wp:
+"\<lbrace>\<lambda>s. invs s \<and> pte = InvalidPTE \<and>
+(\<exists>level asid vref. vs_lookup_slot level asid vref s = Some (level, p) \<and> vref \<in> user_region \<and>
+(\<forall>pt. ako_at (PageTable pt) (table_base p) s \<longrightarrow>
+P (\<lambda>x. if \<exists>level' vref'. vref' \<in> user_region \<and> vref_for_level vref' (level + 1) = vref_for_level vref (level + 1) \<and>
+                                p = pt_slot_offset level (table_base p) vref' \<and>
+                                pt_walk level level' (table_base p) vref' (ptes_of s) = Some (level',x)
+              then (if x = table_base p
+                    then vs_refs_aux level (PageTable (\<lambda>a. if a = table_index p then pte else pt a))
+                    else {})
+              else state_vrefs s x)))
+\<rbrace> store_pte p pte \<lbrace>\<lambda>_ s. P (state_vrefs s)\<rbrace>"
+unfolding store_pte_def set_pt_def
+apply (wpsimp wp: set_object_wp)
+apply (clarsimp simp: fun_upd_def)
+apply (subst state_vrefs_store_NonPageTablePTE)
+apply fastforce+
+apply (clarsimp simp: obj_at_def)
+apply clarsimp
+done
+
+
+definition authorised_page_table_inv :: "'a PAS \<Rightarrow> page_table_invocation \<Rightarrow> bool" where
+  "authorised_page_table_inv aag pti \<equiv>
+   case pti of PageTableMap cap cslot_ptr pde obj_ref \<Rightarrow>
+                 is_subject aag (fst cslot_ptr) \<and> is_subject aag (obj_ref && ~~ mask pt_bits) \<and>
+                 pas_cap_cur_auth aag (ArchObjectCap cap)
+             | PageTableUnmap cap cslot_ptr \<Rightarrow>
+                 is_subject aag (fst cslot_ptr) \<and> aag_cap_auth aag (pasSubject aag) (ArchObjectCap cap)  \<and>
+                 (\<forall>p asid vspace_ref. cap = PageTableCap p (Some (asid, vspace_ref))
+                                      \<longrightarrow> is_subject_asid aag asid \<and>
+                                          (\<forall>x \<in> set [p , p + 2 ^ pte_bits .e. p + 2 ^ pt_bits - 1].
+                                                   is_subject aag (x && ~~ mask pt_bits)))"
 
 lemma store_pte_thread_states[wp]:
   "store_pte p pte \<lbrace>\<lambda>s. P (thread_states s)\<rbrace>"
-  apply (simp add: store_pte_def set_pt_def set_object_def)
-  apply (wp get_object_wp)
-  apply (clarsimp simp: thread_states_def obj_at_def get_tcb_def tcb_states_of_state_def
-                 elim!: rsubst[where P=P, OF _ ext]
-                 split: kernel_object.split_asm option.split)
-  done
+unfolding store_pte_def set_pt_def
+apply (wpsimp wp: set_object_wp)
+  apply (clarsimp simp: get_tcb_def thread_states_def tcb_states_of_state_def obj_at_def
+                 elim!: rsubst[where P=P, OF _ ext])
+done
 
 lemma store_pte_thread_bound_ntfns[wp]:
   "store_pte p pte \<lbrace>\<lambda>s. P (thread_bound_ntfns s)\<rbrace>"
-  apply (simp add: store_pte_def set_pt_def set_object_def)
-  apply (wp get_object_wp)
-  apply (clarsimp simp: thread_bound_ntfns_def obj_at_def get_tcb_def tcb_states_of_state_def
-                 elim!: rsubst[where P=P, OF _ ext]
-                 split: kernel_object.split_asm option.split)
+unfolding store_pte_def set_pt_def
+apply (wpsimp wp: set_object_wp)
+  apply (clarsimp simp: get_tcb_def thread_bound_ntfns_def  obj_at_def
+                 elim!: rsubst[where P=P, OF _ ext])
+done
+
+lemma store_pte_domains_of_state[wp]:
+  "store_pte p pte \<lbrace>\<lambda>s. P (domains_of_state s)\<rbrace>"
+unfolding store_pte_def set_pt_def
+by (wpsimp wp: set_object_wp)
+
+
+lemma mapM_x_store_pte_caps_of_state[wp]:
+  "mapM_x (swp store_pte InvalidPTE) slots \<lbrace>\<lambda>s. P (asid_table s)\<rbrace>"
+  by (wpsimp wp: mapM_x_wp')
+
+lemma state_bits_to_policy_vrefs_subseteq:
+"x \<in> state_bits_to_policy (caps_of_state s) (thread_states s) (thread_bound_ntfns s) (cdt s) X
+\<Longrightarrow> \<forall>x. X x \<subseteq> state_vrefs s x
+\<Longrightarrow>
+ x \<in> state_bits_to_policy (caps_of_state s) (thread_states s) (thread_bound_ntfns s) (cdt s) (state_vrefs s)"
+apply (case_tac x; clarsimp)
+apply (erule state_bits_to_policy.cases)
+apply (fastforce intro: state_bits_to_policy.intros)+
+done
+
+lemma state_asids_to_policy_vrefs_subseteq:
+"x \<in> state_asids_to_policy_aux aag (caps_of_state s) (asid_table s) X
+\<Longrightarrow> \<forall>x. X x \<subseteq> state_vrefs s x
+\<Longrightarrow>
+ x \<in> state_asids_to_policy_aux aag (caps_of_state s) (asid_table s) (state_vrefs s)"
+apply (case_tac x; clarsimp)
+apply (erule state_asids_to_policy_aux.cases)
+apply (fastforce intro: state_asids_to_policy_aux.intros)+
+done
+
+
+lemma store_pte_state_objs_in_policy:
+  "\<lbrace>(\<lambda>s. state_objs_in_policy aag s) and invs
+and (\<lambda>s. (\<exists>slot ref. caps_of_state s slot = Some (ArchObjectCap (PageTableCap (table_base p) ref)))
+\<and>  ((\<exists>asid. vspace_for_asid asid s = Some (table_base p)) \<longrightarrow> table_index p \<notin> kernel_mapping_slots) \<and>
+                table_base p \<notin> global_refs s
+)\<rbrace>
+ store_pte p InvalidPTE
+\<lbrace>\<lambda>_ s. state_objs_in_policy aag s\<rbrace>"
+
+apply (rule hoare_weaken_pre)
+apply (clarsimp simp: state_objs_to_policy_def pred_conj_def)
+apply wps
+apply (rule state_vrefs_store_NonPageTablePTE_wp')
+apply clarsimp
+apply (rule conjI)
+apply clarsimp
+apply (rule exI)+
+apply (rule conjI, assumption)
+apply clarsimp
+
+apply (clarsimp simp: state_objs_to_policy_def)
+apply (erule subsetD)
+apply (clarsimp simp: auth_graph_map_def)
+apply (rule exI, rule conjI, rule refl)+
+apply (erule state_bits_to_policy_vrefs_subseteq)
+apply clarsimp
+apply (clarsimp simp: state_vrefs_def)
+apply (rule exI)
+apply (rule conjI)
+apply (rule_tac x=level in exI)
+apply (rule_tac x="PageTable pt" in exI)
+apply (rule conjI, rule refl)
+
+apply (case_tac "level = asid_pool_level")
+     apply (fastforce dest: vs_lookup_slot_no_asid
+                      simp: ptes_of_Some pts_of_Some aobjs_of_Some pte_of_def obind_def obj_at_def
+                      split: option.splits)
+
+
+apply (subst (asm) vs_lookup_slot_table_unfold)
+apply fastforce+
+apply (fastforce simp: aobjs_of_Some obj_at_def)
+apply (clarsimp simp: vs_refs_aux_def
+graph_of_def)
+apply (clarsimp split: if_splits)
+apply (clarsimp simp: pte_ref2_def)
+apply fastforce
+
+apply (clarsimp simp: state_objs_to_policy_def)
+apply (erule subsetD)
+apply (clarsimp simp: auth_graph_map_def)
+apply (rule exI, rule conjI, rule refl)+
+apply (erule state_bits_to_policy_vrefs_subseteq)
+apply clarsimp
+apply (clarsimp simp: state_vrefs_def)
+apply (rule exI)
+apply (rule conjI)
+apply (rule_tac x=level in exI)
+apply (rule_tac x="PageTable pt" in exI)
+apply (rule conjI, rule refl)
+
+apply (fastforce simp: aobjs_of_Some obj_at_def)
+
+apply (case_tac "level = asid_pool_level")
+     apply (fastforce dest: vs_lookup_table_no_asid
+                      simp: ptes_of_Some pts_of_Some aobjs_of_Some pte_of_def obind_def obj_at_def
+                      split: option.splits)
+apply (drule level_of_table_vs_lookup_table)
+     apply (fastforce dest: vs_lookup_slot_no_asid
+                      simp: ptes_of_Some pts_of_Some aobjs_of_Some pte_of_def obind_def obj_at_def
+                      split: option.splits)+
+apply (simp only:)
+apply (thin_tac "level_of_table _ _ = _")
+apply (clarsimp simp: vs_refs_aux_def
+graph_of_def)
+apply (clarsimp split: if_splits)
+apply (clarsimp simp: pte_ref2_def)
+apply fastforce
+
+done
+
+
+
+lemma store_pte_mapM_x_state_objs_in_policy:
+ "\<lbrace>state_objs_in_policy aag and invs and
+   (\<lambda>s. \<forall>x \<in> set slots. table_base x \<notin> global_refs s \<and> (\<forall>asid. vspace_for_asid asid s \<noteq> Some (table_base x))
+)\<rbrace>
+ mapM_x (swp store_pte InvalidPTE) slots
+\<lbrace>\<lambda>_. state_objs_in_policy aag\<rbrace>"
+apply (rule hoare_strengthen_post)
+apply (rule mapM_x_wp[where S="set slots"])
+
+apply (rule hoare_weaken_pre)
+apply (clarsimp simp: state_objs_to_policy_def pred_conj_def)
+apply (rule hoare_vcg_conj_lift)
+apply wps
+apply (rule state_vrefs_store_NonPageTablePTE_wp')
+   apply (wp store_pte_invs hoare_vcg_const_Ball_lift hoare_vcg_ex_lift hoare_vcg_all_lift)
+apply clarsimp
+   apply (clarsimp simp: wellformed_pte_def)
+apply (rule conjI)
+apply (thin_tac P for P)
+apply clarsimp
+apply (rule exI)+
+apply (rule conjI, assumption)
+apply clarsimp
+
+apply (clarsimp simp: state_objs_to_policy_def)
+apply (erule subsetD)
+apply (clarsimp simp: auth_graph_map_def)
+apply (rule exI, rule conjI, rule refl)+
+apply (erule state_bits_to_policy_vrefs_subseteq)
+apply clarsimp
+apply (clarsimp simp: state_vrefs_def)
+apply (rule exI)
+apply (rule conjI)
+apply (rule_tac x=level in exI)
+apply (rule_tac x="PageTable pt" in exI)
+apply (rule conjI, rule refl)
+
+apply (case_tac "level = asid_pool_level")
+     apply (fastforce dest: vs_lookup_slot_no_asid
+                      simp: ptes_of_Some pts_of_Some aobjs_of_Some pte_of_def obind_def obj_at_def
+                      split: option.splits)
+
+
+apply (subst (asm) vs_lookup_slot_table_unfold)
+apply fastforce+
+apply (fastforce simp: aobjs_of_Some obj_at_def)
+apply (clarsimp simp: vs_refs_aux_def
+graph_of_def)
+apply (clarsimp split: if_splits)
+apply (clarsimp simp: pte_ref2_def)
+apply fastforce
+
+apply (clarsimp simp: state_objs_to_policy_def)
+apply (erule subsetD)
+apply (clarsimp simp: auth_graph_map_def)
+apply (rule exI, rule conjI, rule refl)+
+apply (erule state_bits_to_policy_vrefs_subseteq)
+apply clarsimp
+apply (clarsimp simp: state_vrefs_def)
+apply (rule exI)
+apply (rule conjI)
+apply (rule_tac x=level in exI)
+apply (rule_tac x="PageTable pt" in exI)
+apply (rule conjI, rule refl)
+
+apply (fastforce simp: aobjs_of_Some obj_at_def)
+
+apply (case_tac "level = asid_pool_level")
+     apply (fastforce dest: vs_lookup_table_no_asid
+                      simp: ptes_of_Some pts_of_Some aobjs_of_Some pte_of_def obind_def obj_at_def
+                      split: option.splits)
+apply (drule level_of_table_vs_lookup_table)
+     apply (fastforce dest: vs_lookup_slot_no_asid
+                      simp: ptes_of_Some pts_of_Some aobjs_of_Some pte_of_def obind_def obj_at_def
+                      split: option.splits)+
+apply (simp only:)
+apply (thin_tac "level_of_table _ _ = _")
+apply (clarsimp simp: vs_refs_aux_def
+graph_of_def)
+apply (clarsimp split: if_splits)
+apply (clarsimp simp: pte_ref2_def)
+apply fastforce
+
+apply clarsimp
+
+apply clarsimp
+done
+
+lemma store_pte_state_asids_to_policy:
+  "\<lbrace>(\<lambda>s. state_asids_to_policy aag s \<subseteq> pasPolicy aag) and invs
+and (\<lambda>s. (\<exists>slot ref. caps_of_state s slot = Some (ArchObjectCap (PageTableCap (table_base p) ref)))
+\<and>  ((\<exists>asid. vspace_for_asid asid s = Some (table_base p)) \<longrightarrow> table_index p \<notin> kernel_mapping_slots) \<and>
+                table_base p \<notin> global_refs s
+)\<rbrace>
+ store_pte p InvalidPTE
+\<lbrace>\<lambda>_ s. state_asids_to_policy aag s \<subseteq> pasPolicy aag\<rbrace>"
+apply (rule hoare_weaken_pre)
+apply (clarsimp simp: state_objs_to_policy_def pred_conj_def)
+apply wps
+apply (rule state_vrefs_store_NonPageTablePTE_wp')
+   apply (wpsimp wp: store_pte_invs hoare_vcg_const_Ball_lift hoare_vcg_ex_lift hoare_vcg_all_lift hoare_vcg_imp_lift')
+
+apply (rule conjI)
+apply clarsimp
+
+apply (rule exI)+
+apply (rule conjI, assumption)
+apply clarsimp
+
+apply (erule subsetD)
+apply (erule state_asids_to_policy_vrefs_subseteq)
+apply clarsimp
+apply (clarsimp simp: state_vrefs_def)
+apply (rule exI)
+apply (rule conjI)
+apply (rule_tac x=level in exI)
+apply (rule_tac x="PageTable pt" in exI)
+apply (rule conjI, rule refl)
+
+apply (case_tac "level = asid_pool_level")
+     apply (fastforce dest: vs_lookup_slot_no_asid
+                      simp: ptes_of_Some pts_of_Some aobjs_of_Some pte_of_def obind_def obj_at_def
+                      split: option.splits)
+
+
+apply (subst (asm) vs_lookup_slot_table_unfold)
+apply fastforce+
+apply (fastforce simp: aobjs_of_Some obj_at_def)
+apply (clarsimp simp: vs_refs_aux_def
+graph_of_def)
+apply (clarsimp split: if_splits)
+apply (clarsimp simp: pte_ref2_def)
+apply fastforce
+
+apply (clarsimp)
+apply (erule subsetD)
+apply (erule state_asids_to_policy_vrefs_subseteq)
+apply clarsimp
+apply (clarsimp simp: state_vrefs_def)
+apply (rule exI)
+apply (rule conjI)
+apply (rule_tac x=level in exI)
+apply (rule_tac x="PageTable pt" in exI)
+apply (rule conjI, rule refl)
+
+apply (fastforce simp: aobjs_of_Some obj_at_def)
+
+apply (case_tac "level = asid_pool_level")
+     apply (fastforce dest: vs_lookup_table_no_asid
+                      simp: ptes_of_Some pts_of_Some aobjs_of_Some pte_of_def obind_def obj_at_def
+                      split: option.splits)
+apply (drule level_of_table_vs_lookup_table)
+     apply (fastforce dest: vs_lookup_slot_no_asid
+                      simp: ptes_of_Some pts_of_Some aobjs_of_Some pte_of_def obind_def obj_at_def
+                      split: option.splits)+
+apply (simp only:)
+apply (thin_tac "level_of_table _ _ = _")
+apply (clarsimp simp: vs_refs_aux_def
+graph_of_def)
+apply (clarsimp split: if_splits)
+apply (clarsimp simp: pte_ref2_def)
+apply fastforce
+done
+
+
+lemma store_pte_mapM_x_state_asids_to_policy:
+ "\<lbrace>(\<lambda>s. state_asids_to_policy aag s \<subseteq> pasPolicy aag) and invs
+and (\<lambda>s. \<forall>x \<in> set slots. table_base x \<notin> global_refs s \<and> (\<forall>asid. vspace_for_asid asid s \<noteq> Some (table_base x)))\<rbrace>
+ mapM_x (swp store_pte InvalidPTE) slots
+\<lbrace>\<lambda>_ s. state_asids_to_policy aag s \<subseteq> pasPolicy aag\<rbrace>"
+apply (rule hoare_strengthen_post)
+apply (rule mapM_x_wp[where S="set slots"])
+
+apply (rule hoare_weaken_pre)
+apply (clarsimp simp: state_objs_to_policy_def pred_conj_def)
+apply (rule hoare_vcg_conj_lift)
+apply wps
+apply (rule state_vrefs_store_NonPageTablePTE_wp')
+   apply (wpsimp wp: store_pte_invs hoare_vcg_const_Ball_lift hoare_vcg_ex_lift hoare_vcg_all_lift hoare_vcg_imp_lift')
+apply clarsimp
+   apply (clarsimp simp: wellformed_pte_def)
+apply (rule conjI)
+apply (thin_tac P for P)
+apply clarsimp
+
+apply (rule exI)+
+apply (rule conjI, assumption)
+apply clarsimp
+
+apply (erule subsetD)
+apply (erule state_asids_to_policy_vrefs_subseteq)
+apply clarsimp
+apply (clarsimp simp: state_vrefs_def)
+apply (rule exI)
+apply (rule conjI)
+apply (rule_tac x=level in exI)
+apply (rule_tac x="PageTable pt" in exI)
+apply (rule conjI, rule refl)
+
+apply (case_tac "level = asid_pool_level")
+     apply (fastforce dest: vs_lookup_slot_no_asid
+                      simp: ptes_of_Some pts_of_Some aobjs_of_Some pte_of_def obind_def obj_at_def
+                      split: option.splits)
+
+
+apply (subst (asm) vs_lookup_slot_table_unfold)
+apply fastforce+
+apply (fastforce simp: aobjs_of_Some obj_at_def)
+apply (clarsimp simp: vs_refs_aux_def
+graph_of_def)
+apply (clarsimp split: if_splits)
+apply (clarsimp simp: pte_ref2_def)
+apply fastforce
+
+apply (clarsimp)
+apply (erule subsetD)
+apply (erule state_asids_to_policy_vrefs_subseteq)
+apply clarsimp
+apply (clarsimp simp: state_vrefs_def)
+apply (rule exI)
+apply (rule conjI)
+apply (rule_tac x=level in exI)
+apply (rule_tac x="PageTable pt" in exI)
+apply (rule conjI, rule refl)
+
+apply (fastforce simp: aobjs_of_Some obj_at_def)
+
+apply (case_tac "level = asid_pool_level")
+     apply (fastforce dest: vs_lookup_table_no_asid
+                      simp: ptes_of_Some pts_of_Some aobjs_of_Some pte_of_def obind_def obj_at_def
+                      split: option.splits)
+apply (drule level_of_table_vs_lookup_table)
+     apply (fastforce dest: vs_lookup_slot_no_asid
+                      simp: ptes_of_Some pts_of_Some aobjs_of_Some pte_of_def obind_def obj_at_def
+                      split: option.splits)+
+apply (simp only:)
+apply (thin_tac "level_of_table _ _ = _")
+apply (clarsimp simp: vs_refs_aux_def
+graph_of_def)
+apply (clarsimp split: if_splits)
+apply (clarsimp simp: pte_ref2_def)
+apply fastforce
+
+apply clarsimp
+apply clarsimp
+done
+
+
+lemma mapM_x_store_pte_cdt[wp]:
+  "mapM_x (swp store_pte InvalidPTE) slots \<lbrace>\<lambda>s. P (cdt s)\<rbrace>"
+  by (wpsimp wp: mapM_x_wp')
+
+lemma store_pte_mapM_x_pas_refined:
+ "\<lbrace>pas_refined aag and invs and
+(\<lambda>s. \<forall>x \<in> set slots. table_base x \<notin> global_refs s \<and> (\<forall>asid. vspace_for_asid asid s \<noteq> Some (table_base x)))\<rbrace>
+ mapM_x (swp store_pte InvalidPTE) slots
+\<lbrace>\<lambda>_ s. pas_refined aag s\<rbrace>"
+supply state_asids_to_policy_arch_def[simp del]
+apply (simp add: pas_refined_def)
+apply wpsimp
+apply (rule hoare_vcg_conj_lift, (wpsimp wp: mapM_x_wp_inv ; fail))+
+apply (wpsimp wp: store_pte_mapM_x_state_asids_to_policy store_pte_mapM_x_state_objs_in_policy)
+apply clarsimp
+done
+
+lemma dmo_state_vrefs[wp]:
+  "do_machine_op f \<lbrace>\<lambda>s. P (state_vrefs s)\<rbrace>"
+  by (wpsimp wp: dmo_wp)
+
+lemma dmo_thread_bound_ntfns[wp]:
+  "do_machine_op f \<lbrace>\<lambda>s. P (thread_bound_ntfns s)\<rbrace>"
+  by (wpsimp wp: dmo_wp)
+
+lemma dmo_thread_states[wp]:
+  "do_machine_op f \<lbrace>\<lambda>s. P (thread_states s)\<rbrace>"
+  by (wpsimp wp: dmo_wp)
+
+
+lemma mapM_swp_store_pte_invs_unmap:
+  "\<lbrace>invs and
+    (\<lambda>s.  table_base p \<notin> global_refs s \<and>
+                        (\<forall>asid. vspace_for_asid asid s \<noteq> Some (table_base p))) and
+    K (pte = InvalidPTE)\<rbrace>
+  store_pte p pte \<lbrace>\<lambda>_. invs\<rbrace>"
+   apply simp
+   apply (wp store_pte_invs hoare_vcg_const_Ball_lift hoare_vcg_ex_lift hoare_vcg_all_lift)
+   apply (clarsimp simp: wellformed_pte_def)
   done
+
+(* FIXME ryanb - use for simplifying some lemmas *)
+thm perform_pt_inv_unmap_invs
+
+
+lemma table_base_mask:
+"p && ~~mask b = p \<Longrightarrow>
+       p' && ~~mask b = 0 \<Longrightarrow>
+       (p + p') && ~~mask b = p"
+  by (metis Groups.add_ac(2) VSpaceEntries_AI.neg_mask_add_mask add_left_imp_eq mask_eq_x_eq_0 word_plus_and_or_coroll2)
+
+
+lemma store_pte_pas_refined:
+  "\<lbrace>pas_refined aag and invs
+and (\<lambda>s. (\<exists>slot ref. caps_of_state s slot = Some (ArchObjectCap (PageTableCap (table_base p) ref)))
+\<and>  ((\<exists>asid. vspace_for_asid asid s = Some (table_base p)) \<longrightarrow> table_index p \<notin> kernel_mapping_slots) \<and>
+                table_base p \<notin> global_refs s
+)\<rbrace>
+ store_pte p InvalidPTE
+\<lbrace>\<lambda>_. pas_refined aag\<rbrace>"
+supply state_asids_to_policy_arch_def[simp del]
+apply (clarsimp simp: pas_refined_def)
+apply (wpsimp wp: store_pte_state_objs_in_policy store_pte_state_asids_to_policy)
+done
+
+lemma perform_pt_inv_unmap_pas_refined:
+ "\<lbrace>pas_refined aag and invs and valid_pti (PageTableUnmap cap ct_slot)
+and K (authorised_page_table_inv aag (PageTableUnmap cap ct_slot))\<rbrace>
+            perform_pt_inv_unmap cap ct_slot
+            \<lbrace>\<lambda>_. pas_refined aag\<rbrace>"
+apply (rule hoare_gen_asm)
+term perform_pt_inv_unmap
+apply (unfold perform_pt_inv_unmap_def unmap_page_table_def)
+apply clarsimp
+apply wpsimp
+apply (rule set_cap_pas_refined)
+apply (wpsimp wp: get_cap_wp)
+
+apply (wpsimp wp: hoare_vcg_all_lift)
+apply (rule hoare_vcg_imp_lift')
+
+apply (wpsimp wp: mapM_x_wp_inv)
+
+apply (rule hoare_vcg_conj_lift)
+apply (wp store_pte_mapM_x_pas_refined)
+
+apply (rule hoare_vcg_conj_lift, (wpsimp wp: mapM_x_wp_inv ; fail))+
+
+apply (rule hoare_vcg_conj_lift)
+apply (rule hoare_strengthen_post)
+apply (rule_tac P="valid_vspace_objs and pspace_aligned and valid_asid_table" in mapM_x_wp_inv)
+apply (wpsimp wp: store_pte_InvalidPTE_valid_vspace_objs)
+apply clarsimp
+
+apply (rule hoare_vcg_conj_lift)
+apply (rule hoare_strengthen_post)
+apply (rule_tac
+S="set [acap_obj cap , acap_obj cap + 2 ^ pte_bits .e. acap_obj cap + 2 ^ pt_bits - 1]" and
+P="invs and
+     (\<lambda>s. \<forall>sl\<in>set [acap_obj cap , acap_obj cap + 2 ^ pte_bits .e. acap_obj cap + 2 ^ pt_bits - 1].
+              table_base sl \<notin> global_refs s \<and>
+              (\<forall>asid.
+                  vspace_for_asid asid s \<noteq>
+                  Some (table_base sl)))"
+ in mapM_x_wp)
+apply (rule hoare_pre)
+       apply (wpsimp wp: store_pte_invs hoare_vcg_const_Ball_lift hoare_vcg_ex_lift hoare_vcg_all_lift)
+      apply (clarsimp simp: wellformed_pte_def)
+apply clarsimp
+apply clarsimp
+apply wps
+apply wpsimp
+apply (clarsimp simp: conj_ac)
+apply (strengthen valid_arch_state_asid_table invs_vspace_objs invs_psp_aligned invs_arch_state_strg)+
+apply (clarsimp simp: conj_ac)
+
+
+apply wpsimp
+apply (wpsimp wp: hoare_vcg_imp_lift' hoare_vcg_ball_lift hoare_vcg_all_lift)
+apply clarsimp
+apply wps
+apply (wpsimp wp: static_imp_wp store_pte_invs_unmap store_pte_pas_refined)
+apply (clarsimp simp: conj_ac)
+apply (rule pt_lookup_from_level_wrp)
+apply wpsimp
+apply wpsimp
+apply (clarsimp simp: conj_ac)
+apply (rule conjI)
+apply (prop_tac "acap_map_data cap = None \<longrightarrow> update_map_data cap None = cap")
+apply (clarsimp simp: valid_pti_def update_map_data_def cte_wp_at_caps_of_state)
+apply (case_tac cap; clarsimp)
+apply clarsimp
+apply (clarsimp simp: valid_pti_def cte_wp_at_caps_of_state)
+apply (strengthen valid_arch_state_asid_table invs_vspace_objs invs_psp_aligned invs_arch_state_strg)+
+apply clarsimp
+apply (case_tac cap; clarsimp)
+apply (clarsimp simp: authorised_page_table_inv_def aag_cap_auth_def)
+
+apply clarsimp
+apply (case_tac "cte_wp_at ((=) x) ct_slot s"; clarsimp)
+
+apply (prop_tac "\<forall>sl \<in> set [acap_obj cap , acap_obj cap + 2 ^ pte_bits .e. acap_obj cap + 2 ^ pt_bits - 1].
+table_base sl = acap_obj cap")
+apply (case_tac cap; clarsimp)
+apply (clarsimp simp: valid_pti_def)
+apply (clarsimp simp: cte_wp_at_caps_of_state)
+
+apply (drule (1) caps_of_state_aligned_page_table)
+apply (subst (asm) is_aligned_neg_mask_eq')
+
+apply (drule subsetD[OF upto_enum_step_subset])
+apply clarsimp
+apply (prop_tac "table_base (2^pt_bits - 1) = 0")
+apply (clarsimp simp: and_mask_0_iff_le_mask mask_def)
+apply (prop_tac "table_base x41 \<le> table_base sl")
+  using neg_mask_mono_le apply blast
+apply (prop_tac "table_base sl \<le> table_base (x41 + 2 ^ pt_bits - 1)")
+  using neg_mask_mono_le apply blast
+apply (prop_tac "x41 + 2 ^ pt_bits - 1 = x41 + (2 ^ pt_bits - 1)")
+  apply simp
+apply (simp only: )
+apply (subst (asm) table_base_mask)
+apply simp
+apply simp
+apply simp
+
+
+apply (rule conjI)
+apply clarsimp
+
+
+
+apply (rule conjI)
+apply (case_tac cap; clarsimp)
+apply (clarsimp simp: authorised_page_table_inv_def valid_pti_def cte_wp_at_caps_of_state  aag_cap_auth_def
+                      update_map_data_def cap_auth_conferred_def arch_cap_auth_conferred_def
+cap_links_asid_slot_def cap_links_irq_def)
+apply (clarsimp simp: authorised_page_table_inv_def valid_pti_def)
+apply (clarsimp simp: cte_wp_at_caps_of_state is_transferable.simps)
+apply (rule conjI)
+apply clarsimp
+apply (case_tac cap; clarsimp)
+apply (frule invs_valid_global_refs)
+apply (drule valid_global_refsD)
+apply (fastforce simp: cte_wp_at_caps_of_state)
+apply assumption
+apply (clarsimp simp: cap_range_def)
+apply (case_tac cap; clarsimp)
+apply (clarsimp simp: valid_arch_cap_def)
+
+ apply (frule vspace_for_asid_target)
+   apply (drule valid_vs_lookupD; clarsimp)
+   apply (frule (1) cap_to_pt_is_pt_cap, clarsimp simp: in_omonad obj_at_def)
+    apply (fastforce intro: valid_objs_caps)
+   apply (drule (1) unique_table_refsD[rotated]; clarsimp)
+   apply (clarsimp simp: is_cap_simps)
+
+apply clarsimp
+apply (rule_tac x=a in exI)
+apply clarsimp
+
+apply (case_tac cap; clarsimp)
+apply (clarsimp simp: authorised_page_table_inv_def valid_pti_def cte_wp_at_caps_of_state  aag_cap_auth_def
+                      update_map_data_def cap_auth_conferred_def arch_cap_auth_conferred_def
+cap_links_asid_slot_def cap_links_irq_def is_transferable.simps)
+apply (intro conjI impI)
+
+apply clarsimp
+apply (frule invs_valid_global_refs)
+apply (drule valid_global_refsD)
+apply (fastforce simp: cte_wp_at_caps_of_state)
+apply assumption
+apply (clarsimp simp: cap_range_def)
+
+apply clarsimp
+
+apply (clarsimp simp: valid_arch_cap_def obj_at_def)
+ apply (frule vspace_for_asid_target) back
+   apply (drule valid_vs_lookupD; clarsimp)
+   apply (frule (1) cap_to_pt_is_pt_cap)
+    apply (clarsimp simp: pts_of_Some aobjs_of_Some)
+    apply (fastforce intro: valid_objs_caps)
+   apply (drule (1) unique_table_refsD[rotated]; clarsimp)
+   apply (clarsimp simp: is_cap_simps)
+
+apply clarsimp
+apply (case_tac "level = asid_pool_level")
+apply clarsimp
+apply (drule vs_lookup_slot_no_asid)
+apply (fastforce)+
+apply (intro conjI impI)
+prefer 6
+apply fastforce
+apply (clarsimp simp: valid_arch_cap_def wellformed_mapdata_def)
+apply (subst (asm) vs_lookup_slot_table_unfold)
+apply (fastforce)+
+apply clarsimp
+apply (fastforce dest: reachable_page_table_not_global)
+apply (case_tac ct_slot; clarsimp)
+
+apply (clarsimp simp: valid_arch_cap_def wellformed_mapdata_def)
+apply (subst (asm) vs_lookup_slot_table_unfold)
+apply (fastforce)
+apply (fastforce)
+apply (fastforce)
+apply clarsimp
+
+apply (frule vs_lookup_table_pt_at)
+apply fastforce
+apply fastforce
+apply fastforce
+apply fastforce
+apply fastforce
+
+apply (drule vs_lookup_table_valid_cap)
+apply fastforce
+apply fastforce
+apply fastforce
+apply clarsimp
+
+apply (frule (1) caps_of_state_valid) back
+
+
+apply (case_tac capa; clarsimp)
+apply (case_tac x12; clarsimp)
+apply (clarsimp simp: valid_cap_def obj_at_def)
+apply (clarsimp simp: valid_cap_def obj_at_def)
+apply (clarsimp simp: valid_cap_def obj_at_def)
+apply fastforce
+
+apply (clarsimp simp: valid_arch_cap_def wellformed_mapdata_def)
+apply (subst (asm) vs_lookup_slot_table_unfold)
+apply (fastforce)
+apply (fastforce)
+apply (fastforce)
+apply clarsimp
+  apply (metis AND_twice is_aligned_neg_mask_eq' table_index_max_level_slots vs_lookup_table_vspace)
+
+
+apply (clarsimp simp: valid_arch_cap_def wellformed_mapdata_def)
+apply (subst (asm) vs_lookup_slot_table_unfold)
+apply (fastforce)+
+
+
+apply (case_tac "level = 0"; clarsimp)
+
+apply (frule vs_lookup_table_pt_at)
+apply fastforce+
+
+apply (clarsimp simp: obj_at_def)
+apply (drule valid_vspace_objsD[rotated])
+apply fastforce
+apply (fastforce simp: aobjs_of_Some)
+apply fastforce
+apply (clarsimp simp: ptes_of_Some pts_of_Some aobjs_of_Some)
+apply (erule_tac x="table_index slot" in allE)
+apply (clarsimp simp: is_PageTablePTE_def)
+
+apply (prop_tac "level - 1 < level")
+  using vm_level_not_less_zero apply blast
+
+apply (prop_tac "pt_walk level (level-1) (table_base slot) b (ptes_of s) = Some (level-1, x41)")
+apply (subst pt_walk.simps)
+apply (clarsimp simp: obind_def pte_ref_def2 split: if_splits)
+  using reachable_page_table_not_global vs_lookup_table_extend apply blast
+
+
+apply (clarsimp simp: valid_arch_cap_def obj_at_def)
+ apply (frule vspace_for_asid_target) back
+   apply (drule valid_vs_lookupD; clarsimp)
+   apply (frule (1) cap_to_pt_is_pt_cap)
+    apply (clarsimp simp: pts_of_Some aobjs_of_Some)
+    apply (fastforce intro: valid_objs_caps)
+   apply (drule (1) unique_table_refsD[rotated]; clarsimp)
+   apply (clarsimp simp: is_cap_simps)
+done
+
+
+
+
+lemma state_vrefs_store_PageTablePTE:
+  "\<lbrakk> invs s; is_aligned p pte_bits; vs_lookup_slot level asid vref s = Some (level, p);
+     vref \<in> user_region; is_PageTablePTE pte;  invalid_pte_at p s;
+     pts_of s (the (pte_ref pte)) = Some empty_pt; the (pte_ref pte) \<noteq> table_base p;
+     kheap s (table_base p) = Some (ArchObj (PageTable pt)) \<rbrakk>
+     \<Longrightarrow> state_vrefs (s\<lparr>kheap := \<lambda>a. if a = table_base p
+                                     then Some (ArchObj (PageTable (\<lambda>a. if a = table_index p then pte else pt a)))
+                                     else kheap s a\<rparr>) =
+         (\<lambda>x. if x = table_base p
+              then vs_refs_aux level (PageTable (\<lambda>a. if a = table_index p then pte else pt a))
+              else state_vrefs s x)"
+  apply (rule all_ext)
+
+  apply (case_tac "level = asid_pool_level")
+     apply (clarsimp simp: vs_lookup_slot_def split: if_splits)
+     apply (clarsimp simp: vs_lookup_table_def split: if_splits)
+     apply (drule pool_for_asid_no_pte)
+        apply (simp add: ptes_of_Some pts_of_Some aobjs_of_Some)
+       apply fastforce
+      apply fastforce
+     apply fastforce
+
+apply safe
+
+
+(* first thing *)
+
+   apply (clarsimp simp: state_vrefs_def opt_map_def split: option.splits)
+   apply (case_tac "x = pptr_from_pte pte")
+    (* x = pptr_from_pte pte *)
+  apply clarsimp
+    apply (clarsimp simp: pte_ref_def2)
+    apply (clarsimp split: if_splits)
+    apply (clarsimp simp: vs_refs_aux_def graph_of_def pte_ref2_def)
+      (* x \<noteq> pptr_from_pte pte *)
+   apply (drule_tac s=s and pte=pte and p=p in vs_lookup_PageTablePTE[rotated 9])
+    (* discharging above *)
+               apply (clarsimp simp: pts_of_Some aobjs_of_Some)
+              apply fastforce+
+        apply (rule all_ext)
+        apply (clarsimp simp: opt_map_def pte_of_def obind_def)
+        apply (fastforce dest: pte_ptr_eq)
+       apply simp
+      apply (fastforce simp: opt_map_def)
+     apply (fastforce simp: opt_map_def)
+    apply clarsimp
+(* done *)
+   apply clarsimp
+   apply (drule vs_lookup_level)
+   apply (case_tac "lvl = asid_pool_level")
+    (* lvla = asid_pool_level *)
+    apply clarsimp
+    apply (frule vs_lookup_asid_pool)
+     apply fastforce
+    apply (fastforce simp: asid_pools_of_ko_at obj_at_def)
+    (* lvla \<noteq> asid_pool_level *)
+   apply clarsimp
+   apply (frule vs_lookup_table_pt_at)
+        apply fastforce+
+   apply (clarsimp simp: typ_at_eq_kheap_obj)
+   apply (case_tac "x = table_base p"; clarsimp)
+
+
+    apply (subst (asm) vs_lookup_slot_table)
+     apply clarsimp
+    apply clarsimp
+    apply (prop_tac "is_aligned pt_ptr pt_bits")
+     apply (rule is_aligned_pt[rotated])
+      apply fastforce
+     apply (erule vs_lookup_table_pt_at; fastforce)
+    apply clarsimp
+    apply (drule (1) vs_lookup_table_unique_level; fastforce)
+    (* x \<noteq> table_base p *)
+   apply fastforce
+
+(* second thing *)
+
+  apply (clarsimp simp: state_vrefs_def opt_map_def)
+
+
+   apply (frule vs_lookup_slot_table_base)
+      apply clarsimp+
+
+   apply (case_tac "x = table_base p"; clarsimp)
+
+   apply (drule_tac pte=pte and s'="(s\<lparr>kheap :=
+                                 \<lambda>a. if a = table_base p
+                                      then Some (ArchObj (PageTable (\<lambda>a. if a = table_index p then pte else pt a)))
+                                      else kheap s a\<rparr>)" in vs_lookup_PageTablePTE'[rotated 9])
+            apply fastforce+
+        apply (rule all_ext)
+        apply (clarsimp simp: opt_map_def pte_of_def obind_def)
+        apply (fastforce dest: pte_ptr_eq)
+       apply simp
+      apply (fastforce simp: opt_map_def)
+     apply (fastforce simp: opt_map_def)
+    apply clarsimp
+   apply fastforce
+
+  apply (drule_tac pte=pte and s'="(s\<lparr>kheap :=
+                                \<lambda>a. if a = table_base p
+                                     then Some (ArchObj (PageTable (\<lambda>a. if a = table_index p then pte else pt a)))
+                                     else kheap s a\<rparr>)" in vs_lookup_PageTablePTE'[rotated 9]) back
+           apply fastforce+
+       apply (rule all_ext)
+       apply (clarsimp simp: opt_map_def pte_of_def obind_def)
+       apply (fastforce dest: pte_ptr_eq)
+      apply simp
+     apply (fastforce simp: opt_map_def)
+    apply (fastforce simp: opt_map_def)
+   apply clarsimp
+  apply fastforce
+  done
+
+
+lemma state_vrefs_store_PageTablePTE_wp:
+"\<lbrace>\<lambda>s. invs s \<and> is_PageTablePTE pte \<and> invalid_pte_at p s \<and>
+pts_of s (the (pte_ref pte)) = Some empty_pt \<and> the (pte_ref pte) \<noteq> table_base p \<and>
+(\<exists>level asid vref. vs_lookup_slot level asid vref s = Some (level, p) \<and> vref \<in> user_region \<and>
+(\<forall>pt. ako_at (PageTable pt) (table_base p) s \<longrightarrow>
+P (\<lambda>x. if x = table_base p
+                   then vs_refs_aux level (PageTable (\<lambda>a. if a = table_index p then pte else pt a))
+                   else state_vrefs s x)))
+\<rbrace> store_pte p pte \<lbrace>\<lambda>_ s. P (state_vrefs s)\<rbrace>"
+unfolding store_pte_def set_pt_def
+apply (wpsimp wp: set_object_wp)
+apply (clarsimp simp: fun_upd_def)
+apply (subst state_vrefs_store_PageTablePTE)
+apply fastforce+
+apply (clarsimp simp: obj_at_def)
+apply clarsimp
+done
+
+
+
+
+lemma perform_pt_inv_map_pas_refined[wp]:
+"\<lbrace>pas_refined aag and invs and valid_pti (PageTableMap acap (a, b) pte p)
+and K (authorised_page_table_inv aag (PageTableMap acap (a, b) pte p))\<rbrace>
+            perform_pt_inv_map acap (a,b) pte p
+            \<lbrace>\<lambda>_. pas_refined aag\<rbrace>"
+unfolding perform_pt_inv_map_def
+apply (rule hoare_gen_asm)
+apply_trace wp
+apply (clarsimp simp: pas_refined_def)
+apply (clarsimp simp: state_objs_to_policy_def)
+apply (wps)
+apply (wpsimp wp: state_vrefs_store_PageTablePTE_wp)
+apply (wpsimp wp: arch_update_cap_invs_map  vs_lookup_slot_lift
+hoare_vcg_ex_lift hoare_vcg_all_lift)
+apply (wp hoare_vcg_imp_lift' set_cap_arch_obj_neg)
+apply wps
+apply (wp set_cap_state_vrefs)
+
+apply clarsimp
+apply (clarsimp simp: valid_pti_def)
+apply (clarsimp simp: conj_ac )
+apply (case_tac acap; clarsimp)
+apply (intro conjI impI)
+apply (clarsimp simp: cte_wp_at_caps_of_state)
+apply (clarsimp simp: is_arch_update_def is_arch_cap_def cap_master_cap_def)
+apply (prop_tac "valid_cap cap s")
+apply (rule cte_wp_valid_cap)
+apply (fastforce simp: cte_wp_at_caps_of_state)
+apply fastforce
+apply (case_tac cap; clarsimp)
+apply (case_tac x12; clarsimp)
+apply (case_tac x42; clarsimp)
+apply (clarsimp simp: valid_cap_def cap_aligned_def valid_arch_cap_def)
+
+    apply clarsimp
+    apply (clarsimp simp: vs_lookup_slot_def split: if_splits)
+
+     apply (clarsimp simp: vs_lookup_table_def)
+     apply (clarsimp simp: invalid_pte_at_def)
+     apply (drule pool_for_asid_no_pte)
+        apply (simp)
+       apply fastforce
+      apply fastforce
+     apply simp
+
+    apply clarsimp
+
+    apply (prop_tac "is_aligned ba pt_bits")
+     apply (drule (2) vs_lookup_table_is_aligned)
+        apply fastforce
+       apply fastforce
+      apply fastforce
+     apply clarsimp
+    apply (rename_tac vref' ao pt')
+    apply clarsimp
+    apply (drule (1) vs_lookup_table_target)
+    apply (drule valid_vs_lookupD, erule vref_for_level_user_region; clarsimp)
+    apply (prop_tac "is_pt_cap cap")
+     apply (erule_tac s=s in valid_cap_to_pt_cap[rotated])
+  using pt_at_eq apply blast
+     apply (rule cte_wp_valid_cap)
+      apply (fastforce simp: cte_wp_at_caps_of_state)
+     apply fastforce
+
+    apply (frule (1) cap_to_pt_is_pt_cap, simp, fastforce intro: valid_objs_caps)
+    apply (clarsimp simp: is_cap_simps)
+    apply (clarsimp simp: cte_wp_at_caps_of_state)
+    apply (clarsimp simp: is_arch_update_def cap_master_cap_def split: cap.splits arch_cap.splits option.splits)
+
+    apply (drule (1) unique_table_refsD[rotated])
+      apply clarsimp
+     apply fastforce
+    apply (clarsimp simp: table_cap_ref_def)
+
+apply (erule cte_wp_at_weakenE)
+apply clarsimp
+apply (case_tac c; clarsimp)
+apply (clarsimp simp: vs_cap_ref_def vs_cap_ref_arch_def split: arch_cap.splits)
+apply (clarsimp simp: is_arch_update_def cap_master_cap_def)
+
+
+apply (rule_tac x=level in exI)
+apply (rename_tac asid ao)
+apply (rule_tac x=asid in exI)
+apply (rule_tac x=vref in exI)
+apply clarsimp
+
+apply (intro conjI impI; (fastforce | (clarsimp simp: pas_refined_def; fail))?)
+apply clarsimp
+  using Invariants_AI.cte_wp_at_cte_at apply blast
+
+apply clarsimp
+apply (erule state_asids_to_policy_aux.cases)
+  using Invariants_AI.cte_wp_at_cte_at apply blast
+  using Invariants_AI.cte_wp_at_cte_at apply blast
+  using Invariants_AI.cte_wp_at_cte_at apply blast
+  using Invariants_AI.cte_wp_at_cte_at apply blast
+
+apply (clarsimp split: if_splits)
+apply (clarsimp simp: pas_refined_def)
+apply (erule state_irqs_to_policy_aux.cases)
+apply (clarsimp split: if_splits)
+apply (fastforce dest: sita_controlled)
+
+(* state_asids_to_policy *)
+apply clarsimp
+apply (erule state_asids_to_policy_aux.cases)
+
+apply (clarsimp simp: cte_wp_at_caps_of_state)
+apply (clarsimp split: if_splits)
+
+apply (clarsimp simp: authorised_page_table_inv_def)
+apply (clarsimp simp: aag_cap_auth_def cap_auth_conferred_def arch_cap_auth_conferred_def cap_links_asid_slot_def label_owns_asid_slot_def)
+apply (clarsimp simp: pas_refined_def)
+apply (erule subsetD) back
+thm sata_asid
+apply (fastforce dest: sata_asid)
+apply clarsimp
+apply (clarsimp split: if_splits)
+prefer 2
+apply (fastforce simp: pas_refined_def dest: subsetD dest!: sata_asid_lookup)
+apply (clarsimp simp: vs_refs_aux_def)
+apply (fastforce simp: pas_refined_def dest: subsetD dest!: state_asids_to_policy_aux.intros)
+
+apply clarsimp
+apply (clarsimp simp: cte_wp_at_caps_of_state)
+apply (clarsimp simp: auth_graph_map_def)
+apply (erule state_bits_to_policy.cases)
+(* sbta_caps *)
+apply (clarsimp simp: is_arch_update_def cap_master_cap_def split: cap.splits arch_cap.splits option.splits)
+apply (clarsimp simp: pas_refined_def)
+apply (erule subsetD)
+apply (clarsimp simp: auth_graph_map_def state_objs_to_policy_def)
+apply (clarsimp split: if_splits)
+apply (fastforce dest: sbta_caps simp: cap_auth_conferred_def arch_cap_auth_conferred_def)
+apply (fastforce dest: sbta_caps simp: cap_auth_conferred_def arch_cap_auth_conferred_def)
+(* sbta_untyped *)
+apply (clarsimp simp: is_arch_update_def cap_master_cap_def split: cap.splits arch_cap.splits option.splits)
+apply (clarsimp simp: pas_refined_def)
+apply (erule subsetD)
+apply (clarsimp simp: auth_graph_map_def state_objs_to_policy_def)
+apply (clarsimp split: if_splits)
+apply (fastforce dest: sbta_untyped)
+(* sbta_ts *)
+apply (clarsimp simp: is_arch_update_def cap_master_cap_def split: cap.splits arch_cap.splits option.splits)
+apply (clarsimp simp: pas_refined_def)
+apply (erule subsetD)
+apply (clarsimp simp: auth_graph_map_def state_objs_to_policy_def)
+apply (fastforce dest: sbta_ts)
+(* sbta_bounds *)
+apply (clarsimp simp: is_arch_update_def cap_master_cap_def split: cap.splits arch_cap.splits option.splits)
+apply (clarsimp simp: pas_refined_def)
+apply (erule subsetD)
+apply (clarsimp simp: auth_graph_map_def state_objs_to_policy_def)
+apply (fastforce dest: sbta_bounds)
+(* sbta_cdt *)
+apply (clarsimp simp: is_arch_update_def cap_master_cap_def split: cap.splits arch_cap.splits option.splits)
+apply (clarsimp simp: pas_refined_def)
+apply (erule subsetD)
+apply (clarsimp simp: auth_graph_map_def state_objs_to_policy_def)
+apply (clarsimp split: if_splits)
+apply (rule exI, rule conjI, rule refl)+
+apply (drule_tac caps="caps_of_state s" in sbta_cdt)
+apply simp
+apply clarsimp
+apply (fastforce elim: is_transferable.cases)
+apply fastforce
+apply (rule exI, rule conjI, rule refl)+
+apply (drule_tac caps="caps_of_state s" in sbta_cdt)
+apply simp
+apply clarsimp
+apply (fastforce elim: is_transferable.cases)
+(* sbta_cdt_transferable *)
+apply (clarsimp simp: is_arch_update_def cap_master_cap_def split: cap.splits arch_cap.splits option.splits)
+apply (clarsimp simp: pas_refined_def)
+apply (erule subsetD)
+apply (clarsimp simp: auth_graph_map_def state_objs_to_policy_def)
+apply (fastforce dest: sbta_cdt_transferable)
+(* sbta_vref *)
+apply (clarsimp split: if_splits)
+prefer 2
+apply (clarsimp simp: is_arch_update_def cap_master_cap_def split: cap.splits arch_cap.splits option.splits)
+apply (clarsimp simp: pas_refined_def)
+apply (erule subsetD)
+apply (clarsimp simp: auth_graph_map_def state_objs_to_policy_def)
+apply (fastforce dest: sbta_vref)
+
+apply (clarsimp simp: authorised_page_table_inv_def)
+
+apply (clarsimp simp: vs_refs_aux_def graph_of_def)
+apply (case_tac pte; clarsimp)
+apply (clarsimp simp: pte_ref2_def aag_cap_auth_def cap_auth_conferred_def arch_cap_auth_conferred_def)
+apply (case_tac "aa = table_index p"; clarsimp)
+
+
+apply (clarsimp simp: is_arch_update_def cap_master_cap_def split: cap.splits arch_cap.splits option.splits)
+apply (clarsimp simp: pas_refined_def)
+apply (erule subsetD)
+apply (clarsimp simp: auth_graph_map_def state_objs_to_policy_def)
+apply (rule_tac x="table_base p" in exI, rule conjI)
+apply simp
+apply (rule exI, rule conjI, rule refl)
+apply (rule sbta_vref)
+apply (clarsimp simp: state_vrefs_def)
+thm sbta_vref
+
+apply (case_tac "level = asid_pool_level")
+    apply (clarsimp simp: vs_lookup_slot_def split: if_splits)
+
+     apply (clarsimp simp: vs_lookup_table_def)
+     apply (clarsimp simp: invalid_pte_at_def)
+     apply (drule pool_for_asid_no_pte)
+        apply (simp)
+       apply fastforce
+      apply fastforce
+     apply simp
+
+apply clarsimp
+apply (drule vs_lookup_slot_table_base)
+apply clarsimp+
+
+apply (rule exI, rule conjI)
+apply (rule exI, rule exI)
+apply (rule conjI, rule refl)
+apply (rule exI)+
+apply (rule conjI, assumption)
+apply (simp add: obj_at_def aobjs_of_Some)
+apply (clarsimp simp: vs_refs_aux_def graph_of_def)
+apply (rule exI)+
+apply (clarsimp simp: pte_ref2_def)
+apply fastforce
+done
+
+
+
+(* FIXME ryanb: resume *)
+lemma perform_page_table_invocation_pas_refined:
+  "\<lbrace>pas_refined aag and invs and valid_pti iv
+and K (authorised_page_table_inv aag iv)\<rbrace> perform_page_table_invocation iv \<lbrace>\<lambda>_. pas_refined aag\<rbrace>"
+unfolding perform_page_table_invocation_def
+apply wpsimp
+apply (wpsimp wp: perform_pt_inv_unmap_pas_refined perform_pt_inv_map_pas_refined)+
+apply (case_tac iv; clarsimp)
+done
+
+
 
 lemma auth_graph_map_def2:
   "auth_graph_map f S = (\<lambda>(x, auth, y). (f x, auth, f y)) ` S"
@@ -419,34 +2221,6 @@ lemma store_pte_ekheap[wp]:
   apply simp
   done
 
-crunch asid_table_inv [wp]: store_pte "\<lambda>s. P (asid_table s)"
-
-lemma store_pte_pas_refined[wp]:
-  "\<lbrace>pas_refined aag and
-    K (\<forall>x level. pte_ref2 level pte = Some x
-           \<longrightarrow> (\<forall>a \<in> snd (snd x). \<forall>p' \<in> (ptr_range (fst x) (fst (snd x))).
-                auth_graph_map (pasObjectAbs aag) {(p && ~~ mask pt_bits, a, p')} \<subseteq> pasPolicy aag))\<rbrace>
-   store_pte p pte
-   \<lbrace>\<lambda>rv. pas_refined aag\<rbrace>"
-  sorry
-(* FIXME ryanb
-  apply (simp add: auth_graph_map_def2)
-  apply (simp add: pas_refined_def state_objs_to_policy_def)
-  apply (rule hoare_pre)
-   apply (wp tcb_domain_map_wellformed_lift | wps)+
-  apply clarsimp
-  apply (rule conjI)
-   apply (clarsimp dest!: auth_graph_map_memD split del: if_split)
-   apply (erule state_bits_to_policy.cases,
-          auto intro: state_bits_to_policy.intros auth_graph_map_memI
-               split: if_split_asm)[1]
-  apply (erule_tac B="state_asids_to_policy_aux _ _ _ _" in subset_trans[rotated])
-  apply (auto intro: state_asids_to_policy_aux.intros
-              elim!: state_asids_to_policy_aux.cases
-               elim: subset_trans[rotated]
-              split: if_split_asm)
-  done
-*)
 
 lemma set_asid_pool_st_vrefs[wp]:
   "\<lbrace>\<lambda>s. P ((state_vrefs s) (p := (\<lambda>(r, p). (p, ucast r, AASIDPool, Control)) ` graph_of pool))\<rbrace>
@@ -458,7 +2232,7 @@ lemma set_asid_pool_st_vrefs[wp]:
                         vs_refs_aux_def
                  split: kernel_object.split_asm arch_kernel_obj.split_asm
                  elim!: rsubst[where P=P, OF _ ext])
-  sorry
+  oops
 
 lemma set_asid_pool_thread_states[wp]:
   "set_asid_pool p pool \<lbrace>\<lambda>s. P (thread_states s)\<rbrace>"
@@ -497,6 +2271,7 @@ lemma set_asid_pool_pas_refined[wp]:
   apply (simp add: pas_refined_def state_objs_to_policy_def)
   apply (rule hoare_pre)
    apply (wp tcb_domain_map_wellformed_lift | wps)+
+(*
   apply clarsimp
   apply (rule conjI)
    apply (clarsimp dest!: auth_graph_map_memD)
@@ -507,7 +2282,8 @@ lemma set_asid_pool_pas_refined[wp]:
                simp: subsetD[OF _ state_asids_to_policy_aux.intros(2)]
               elim!: state_asids_to_policy_aux.cases
               split: if_split_asm)
-  sorry
+*)
+  oops
 (* FIXME ryanb
   apply fastforce+
   done
@@ -517,7 +2293,7 @@ lemma pas_refined_clear_asid:
   "pas_refined aag s
    \<Longrightarrow> pas_refined aag (s\<lparr>arch_state := arch_state s\<lparr>riscv_asid_table := \<lambda>a. if a = asid then None
                                                                              else asid_table s a\<rparr>\<rparr>)"
-  sorry
+  oops
 (* FIXME ryanb
   by (fastforce simp: pas_refined_def state_objs_to_policy_def
                intro: state_asids_to_policy_aux.intros
